Homework answers
================

1A)

  1) 4.76 * 10^-4
  2) 0.000064
  3) 0.028

2A)

  1) b^2 - 3b = b(b - 3)
  2) 108(a^6)(d^8)
  3) abc + ad
  4) a^3 + ab - (a^2)b - b^2
  5)

     a) x(y - z)
     b) a(b + 1)
     c) y(a + 1)
     d) bcde(a + 1)

  6) 4b - 2a

3A)

  1) 5a - 4 = 2a + 5
     5a - 2a -4 = 2a - 2a + 5
     3a - 4 = 5
     3a -4 + 4 = 5 + 4
     3a = 9
     3a/3 = 9/3
     a = 3

  2) 3(y - 2) = 5y + 6
     3y - 6 = 5y + 6
     3y - 5y - 6 = 5y - 5y + 6
     -2y - 6 = 6
     -2y - 6 + 6 = 6 + 6
     -2y = 12
     -2y/-2 = 12/-2
     y = -6

4A)

  1) 2x + 3y = 5
     5x - 4y = -22

     8x + 12y = 20
     15x - 12y = -66

     23x = -46
     x = -2

  2) 2g - 3h = 1
     3g - 4h = 7

     -8g + 12h = -4
     9g - 12h = 21

     g = 17

Workbook 2

1A)

  1) 4.76 * 10^-4
  2) 0.000064
  3) 0.028

2A)

  1) b^2 - 3b = b(b - 3)
  2) 108(a^6)(d^8)
  3) abc + ad
  4) a^3 + ab - (a^2)b - b^2
  5)

     a) x(y - z)
     b) a(b + 1)
     c) y(a + 1)
     d) bcde(a + 1)

  6) 4b - 2a

3A)

  1) 5a - 4 = 2a + 5
     5a - 2a -4 = 2a - 2a + 5
     3a - 4 = 5
     3a -4 + 4 = 5 + 4
     3a = 9
     3a/3 = 9/3
     a = 3

  2) 3(y - 2) = 5y + 6
     3y - 6 = 5y + 6
     3y - 5y - 6 = 5y - 5y + 6
     -2y - 6 = 6
     -2y - 6 + 6 = 6 + 6
     -2y = 12
     -2y/-2 = 12/-2
     y = -6

4A)

  1) 2x + 3y = 5
     5x - 4y = -22

     8x + 12y = 20
     15x - 12y = -66

     23x = -46
     x = -2

     2x + 3y = 5
     -4 + 3y = 5
     3y = 9
     y = 3

  2) 2g - 3h = 1
     3g - 4h = 7

     -8g + 12h = -4
     9g - 12h = 21

     g = 17

     2g - 3h = 1
     34 - 3h = 1
     -3h = -33
     h = 11

1B)
  1) 7.76 * 10^-3
  2) 0.348
  3) 0.0042

2B)
  1) -2ac - a^2 = a(-2c - a)
  2) 81(a^8)(b^4) * -2a^3b^6
     = -162(a^11)(b^10)
  3) 2stc + sd
  4) 2(a^3) + 6ab -c(a^2) - 3bc
  5)

     a) a(b + c)
     b) r(s - 1)
     c) t(2a + 1)
     d) xy(2yz + x)

  6) a + 8b

3B)
  1) 7a + 8 = 9a - 3
     7a + 8 - 7a = 9a - 7a - 3
     8 = 2a - 3
     8 + 3 = 2a - 3 + 3
     11 = 2a
     11 / 2 = 2a / 2
     a = 5.5
  2) 3(2y - 1) = 4y - 6
     6y - 3 = 4y - 6
     6y - 3 - 4y = 4y - 6 - 4y
     2y - 3 = -6
     2y - 3 + 3 = -6 + 3
     2y = -3
     2y / 2 = -3 / 2
     y = -1.5

4B)
  1) 2x + 3y = 10
     5x - 5y = -50

     10x + 15y = 50
     15x - 15y = -150

     25x = -100
     x = -4

     2x + 3y = 10
     2(-4) + 3y = 10
     3y - 8 = 10
     3y = 18
     y = 6
  2) 7p - 2q = 3
     3p + 8q = -43

     28p - 8q = 12
     3p + 8q = -43

     31p = -31
     p = -1

     7p - 2q = 3
     -7 - 2q = 3
     -2q = 10
     q = -5
